Launchbury/CallArityEtaExpand.thy
@@ -20,7 +20,7 @@ begin
   interpretation AbstractTransformBoundSubst
     "\<lambda> a . inc\<cdot>a"
     "\<lambda> a . pred\<cdot>a"
-    "\<lambda> \<Delta> e a . (a, ccFix \<Delta>\<cdot>(cccExp e\<cdot>a))"
+    "\<lambda> \<Delta> e a . (a, combined_restrict (domA \<Delta>) (ccFix \<Delta>\<cdot>(cccExp e\<cdot>a)))"
     "\<lambda> b . fst b"
     "\<lambda> b . fst (snd b)"
     "Aeta_expand"
