Launchbury/CallFutures.thy
@@ -1,0 +1,145 @@
+theory CallFutures
+imports Vars "Nominal-Utils" "Set_Cpo"
+begin
+
+type_synonym future = "var \<Rightarrow> nat"
+
+definition no_future :: future where "no_future v = 0"
+
+definition possible :: "var \<Rightarrow> future \<Rightarrow> bool"
+  where "possible v f = (f v > 0)"
+
+inductive_set domF :: "future \<Rightarrow> var set" for f
+  where "possible v f \<Longrightarrow> v \<in> domF f"
+
+lemma possible_eqvt[eqvt]: "\<pi> \<bullet> possible v f = possible (\<pi> \<bullet> v) (\<pi> \<bullet> f)"
+  unfolding possible_def by simp
+
+definition after :: "var \<Rightarrow> future \<Rightarrow> future"
+  where "after v f = (f(v := f v - 1))"
+
+lemma after_eqvt[eqvt]: "\<pi> \<bullet> after v f = after (\<pi> \<bullet> v) (\<pi> \<bullet> f)"
+  unfolding after_def by simp
+
+lemma after_swap: "after x (after y f) = after y (after x f)"
+  unfolding after_def by auto
+
+definition without :: "var \<Rightarrow> future \<Rightarrow> future"
+  where "without v f = (f(v := 0))"
+
+lemma without_eqvt[eqvt]: "\<pi> \<bullet> without v f = without (\<pi> \<bullet> v) (\<pi> \<bullet> f)"
+  unfolding without_def by simp
+
+
+type_synonym futures = "var \<Rightarrow> future set"
+
+definition combine :: "future \<Rightarrow> future \<Rightarrow> future"
+  where "combine f1 f2 v = f1 v + f2 v"
+
+(* http://stackoverflow.com/questions/16603886/inductive-set-with-non-fixed-parameters *)
+
+inductive paths' :: "futures \<Rightarrow> future set \<Rightarrow> var list \<Rightarrow> bool" for G
+  where "paths' G current []"
+  | "f \<in> current \<Longrightarrow> possible x f \<Longrightarrow> paths' G (combine (after x f) ` (G x)) path \<Longrightarrow> paths' G current (x#path)"
+
+definition paths  :: "futures \<Rightarrow> future set \<Rightarrow> var list set" 
+  where "paths G current = Collect (paths' G current)"
+lemma elim_paths'[pred_set_conv]: "paths' G f p \<longleftrightarrow> p \<in> paths G f" unfolding paths_def by simp
+
+lemmas paths_intros[intro?] = paths'.intros[unfolded elim_paths']
+lemmas paths_induct[consumes 1, induct set: paths] = paths'.induct[to_set]
+lemmas paths_cases[consumes 1, cases set: paths] = paths'.cases[to_set]
+lemmas paths_simpss = paths'.simps[to_set]
+
+lemma possible_no_future[simp]: "possible xa no_future \<longleftrightarrow> False"
+  by (auto simp add: possible_def no_future_def)
+
+lemma possible_upd[simp]: "possible x' (f(x := n)) \<longleftrightarrow> (x = x' \<and> n > 0) \<or> (possible x' f \<and> x' \<noteq> x)"
+  by (auto simp add: possible_def no_future_def)
+
+lemma after_upd[simp]: "after x (f(x := n)) = f(x := n - 1)"
+  by (auto simp add: after_def)
+
+lemma [simp]: "x \<noteq> y \<Longrightarrow> after x (f(y := n)) =( after x f)(y := n)"
+  by (auto simp add: after_def)
+
+lemma no_future_upd0[simp]: "no_future(x := 0) = no_future"
+  by (auto simp add: no_future_def)
+
+lemma combine_nofuture[simp]: "combine no_future f = f"
+  by (auto simp add: no_future_def combine_def)
+
+definition may_call :: "var \<Rightarrow> future set \<Rightarrow> future set"
+  where "may_call v fs = {f . \<exists> f' \<in> fs. \<forall> x. x \<noteq> v \<longrightarrow> f x = f' x}"
+
+lemma may_call_cont: "cont (may_call v)" sorry
+lemmas may_call_cont[cont2cont, simp]
+
+
+text {* Some tests *}
+
+lemma cons_eq_replicate[simp]: "x'#xs = replicate n x \<longleftrightarrow> x' = x \<and> n > 0 \<and> xs = replicate (n - 1) x"
+  by (cases n) auto
+
+lemma snoc_eq_replicate[simp]: "xs @ [x'] = replicate n x  \<longleftrightarrow> x' = x \<and> n > 0 \<and> xs = replicate (n - 1) x"
+proof-
+  have "xs @ [x'] = replicate n x \<longleftrightarrow> rev (xs @ [x']) = rev (replicate n x)" by (metis rev_rev_ident)
+  also have "\<dots> \<longleftrightarrow> rev (xs @ [x']) = replicate n x" by (metis rev_replicate)
+  also have "\<dots> \<longleftrightarrow> x'# (rev xs)  = replicate n x" by (metis rev.simps(2) rev_rev_ident)
+  also have "\<dots> \<longleftrightarrow> x' = x \<and> n > 0 \<and> rev xs = replicate (n - 1) x" by (rule cons_eq_replicate)
+  also have "\<dots> \<longleftrightarrow> x' = x \<and> n > 0 \<and> xs = replicate (n - 1) x" by (metis rev_rev_ident rev_replicate)
+  finally show ?thesis.
+qed 
+
+lemma [simp]: "replicate n x @ [x'] = replicate n' x \<longleftrightarrow> n' = Suc n \<and> x' = x"
+  by auto
+
+lemma
+  fixes G current
+  assumes [simp]:"G = ((\<lambda> _. {})(x := current))"
+  assumes [simp]:"current = {no_future(x := 1)}"
+  shows "paths G current = {replicate n x | n. True}"
+proof(rule set_eqI, rule)
+  fix p
+  assume "p \<in> paths G current"
+  from  this `current = _` 
+  show "p \<in> {replicate n x |n. True}" by (induction) auto
+next
+  fix p
+  assume "p \<in> {replicate n x |n. True}"
+  then obtain n where "p = replicate n x" by auto
+  thus "p \<in> paths G current"
+  by (induction p arbitrary: n)(auto intro: paths_intros)
+qed   
+
+lemma
+  assumes [simp]: "x\<noteq>y"
+  assumes [simp]:"G = ((\<lambda> _. {})(x := current, y := {no_future}))"
+  assumes [simp]:"current = {no_future(x := 1), no_future(y := 1)}"
+  shows "paths G current = {replicate n x | n. True} \<union> {replicate n x @ [y]| n. True}"
+proof(rule set_eqI, rule)
+  fix p
+  assume "p \<in> paths G current"
+  hence "(current = {no_future} \<Longrightarrow> p = [])" and "current = {no_future(x := 1), no_future(y := 1)} \<Longrightarrow> p \<in> {replicate n x | n. True} \<union>  {replicate n x @ [y]| n. True}"
+    by induction (auto, arith+)
+  with `current = _`
+  show "p \<in> {replicate n x | n. True} \<union>  {replicate n x @ [y]| n. True}" by blast
+next
+  fix p
+  {
+  fix n
+  have "replicate n x \<in> paths G current"
+    by (induction n) (auto intro: paths_intros (1) paths_intros(2)[where f = "no_future(x := Suc 0)"])
+  moreover
+  have "replicate n x @ [y] \<in> paths G current"
+    by (induction n) (auto intro: paths_intros(1) paths_intros(2)[where f = "no_future(x := Suc 0)"]  paths_intros(2)[where f = "no_future(y := Suc 0)"])
+  moreover
+  note calculation
+  }
+  moreover
+  assume  "p \<in> {replicate n x | n. True} \<union>  {replicate n x @ [y]| n. True}"
+  ultimately
+  show "p \<in> paths G current" by blast
+qed
+
+end
