Launchbury/CoCallsFuture.thy
@@ -1,0 +1,18 @@
+theory CoCallsFuture
+imports CoCallGraph CallFutures
+begin
+
+inductive_set any_future :: "var set \<Rightarrow> future set" for S
+  where "domF f \<subseteq> S \<Longrightarrow> f \<in> any_future S"
+
+definition conformsToCC :: "future \<Rightarrow> CoCalls \<Rightarrow> bool"
+  where "conformsToCC f G \<longleftrightarrow> (\<forall>x y. (x--y\<notin>G) \<longrightarrow> possible x f \<longrightarrow>  \<not> possible y (after x f))"
+
+definition ccFilterFuture  :: "future set \<Rightarrow> CoCalls \<Rightarrow> future set"
+  where "ccFilterFuture S G = {f \<in> S . conformsToCC f G}"
+
+lemma no_future_conforms:  "conformsToCC no_future G"
+  unfolding conformsToCC_def by simp
+
+
+end  
