Launchbury/FutureEtaExpand.thy
@@ -1,0 +1,343 @@
+theory FutureEtaExpand
+imports CallFutures AEnv Terms EtaExpansionArity EtaExpansionSestoft AbstractTransform Set_Cpo_Nominal  Sestoft SestoftGC
+begin
+
+default_sort type
+
+type_synonym oneShot = "one"
+abbreviation notOneShot :: oneShot where "notOneShot \<equiv> ONE"
+abbreviation oneShot :: oneShot where "oneShot \<equiv> \<bottom>"
+
+type_synonym two = "oneShot\<^sub>\<bottom>"
+abbreviation many :: two where "many \<equiv> up\<cdot>notOneShot"
+abbreviation once :: two where "once \<equiv> up\<cdot>oneShot"
+abbreviation none :: two where "none \<equiv> \<bottom>"
+
+definition two_pred where "two_pred = (\<Lambda> x. if x = once then \<bottom> else x)"
+
+definition record_call where "record_call x = (\<Lambda> ce. (\<lambda> y. if x = y then two_pred\<cdot>(ce y) else ce x))"
+
+lemma two_conj: "c = many \<or> c = once \<or> c = none" sorry
+
+lemma two_cases[case_names many once none]:
+  obtains "c = many" | "c = once" | "c = none" using two_conj by metis
+
+
+definition abstractPath :: "var list set \<Rightarrow> var \<Rightarrow> two"
+  where "abstractPath ps v = undefined"
+
+text {* Expands only if it is safe to do so, i.e. either one-shot or already a function. *}
+
+fun rhsExpand :: "(Arity \<times> one) \<Rightarrow> exp \<Rightarrow> exp"
+  where "rhsExpand (a,c) e = (if isLam e \<or> c = \<bottom> then Aeta_expand a e else e)"
+
+interpretation supp_bounded_transform rhsExpand sorry
+
+lemma rhsExpand[eqvt]: "\<pi> \<bullet> rhsExpand = rhsExpand" sorry
+
+
+fun Astack :: "stack \<Rightarrow> Arity"
+  where "Astack [] = 0"
+      | "Astack (Arg x # S) = inc\<cdot>(Astack S)"
+      | "Astack (Upd x # S) = 0"
+      | "Astack (Dummy x # S) = 0"
+
+
+lemma Aeta_expand_correct:
+  assumes "Astack S \<sqsubseteq> a"
+  shows "(\<Gamma>, Aeta_expand a e, S) \<Rightarrow>\<^sup>* (\<Gamma>, e, S)"
+proof-
+  have "arg_prefix S = Rep_Arity (Astack S)"
+    by (induction S arbitrary: a rule: arg_prefix.induct) (auto simp add: Arity.zero_Arity.rep_eq[symmetric])
+  also
+  from assms(1)
+  have "Rep_Arity a \<le> Rep_Arity (Astack S)" by (metis below_Arity.rep_eq)
+  finally
+  show ?thesis by transfer (rule eta_expansion_correct')
+qed
+
+
+fun restr_stack :: "var set \<Rightarrow> stack \<Rightarrow> stack"
+  where "restr_stack V [] = []"
+      | "restr_stack V (Arg x # S) = Arg x # restr_stack V S"
+      | "restr_stack V (Upd x # S) = (if x \<in> V then Upd x # restr_stack V S else restr_stack (insert x V) S)"
+      | "restr_stack V (Dummy x # S) = Dummy x # restr_stack V S"
+
+lemma Astack_restr_stack_below:
+  "Astack (restr_stack V S) \<sqsubseteq> Astack S"
+  by (induction V S rule: restr_stack.induct) auto
+
+
+
+definition fup_fst :: "(var \<Rightarrow> (Arity \<times> one)\<^sub>\<bottom>) \<Rightarrow> AEnv"
+    where "fup_fst e x = fup\<cdot>(\<Lambda> p. up\<cdot>(cfst\<cdot>p))\<cdot>(e x)"
+
+lemma fup_fst_eqvt[eqvt]: "\<pi> \<bullet> (fup_fst e x) = fup_fst (\<pi> \<bullet> e) (\<pi> \<bullet> x)"
+  unfolding fup_fst_def
+  by perm_simp rule
+
+locale FutureAnalysis =
+  fixes aExp :: "exp \<Rightarrow> Arity \<rightarrow> AEnv"
+  fixes fExp :: "exp \<Rightarrow> Arity \<rightarrow> future set"
+  fixes fHeap :: "heap \<Rightarrow> (AEnv \<times> future set) \<rightarrow> (var \<Rightarrow> (Arity \<times> one)\<^sub>\<bottom>)"
+
+  assumes aExp_Var: "up \<cdot> n \<sqsubseteq> (aExp (Var x)\<cdot>n) x"
+  assumes aExp_App: "aExp (App e x) \<cdot> n = aExp e \<cdot>(inc\<cdot>n) \<squnion> AE_singleton x \<cdot> (up\<cdot>0)"
+  assumes aExp_subst_App_Lam: "aExp (e[y::=x]) \<sqsubseteq> aExp (App (Lam [y]. e) x)"
+  assumes aExp_Lam: "aExp (Lam [y]. e) \<cdot> n = env_delete y (aExp e \<cdot>(pred\<cdot>n))"
+
+
+  assumes fExp_App: "fExp (App e x)\<cdot>n = may_call x (fExp e \<cdot>(inc\<cdot>n))"
+
+  assumes aExp[eqvt]: "\<pi> \<bullet> aExp = aExp"
+  assumes fExp[eqvt]: "\<pi> \<bullet> fExp = fExp"
+  assumes fHeap[eqvt]: "\<pi> \<bullet> fHeap = fHeap"
+begin
+
+  sublocale AbstractTransformBound
+    "\<lambda> a . inc\<cdot>a"
+    "\<lambda> a . pred\<cdot>a"
+    "\<lambda> \<Delta> e a . (a, fHeap \<Delta>\<cdot>(aExp e\<cdot>a, fExp e\<cdot>a))"
+    "fst"
+    "\<lambda> b . fup_fst (snd b)"
+    "rhsExpand"
+    "snd"
+  apply default
+  apply (((rule eq_reflection)?, perm_simp, rule)+)[7]
+  done
+
+  sublocale AbstractTransformBoundSubst
+    "\<lambda> a . inc\<cdot>a"
+    "\<lambda> a . pred\<cdot>a"
+    "\<lambda> \<Delta> e a . (a, fHeap \<Delta>\<cdot>(aExp e\<cdot>a, fExp e\<cdot>a))"
+    "fst"
+    "\<lambda> b . fup_fst (snd b)"
+    "rhsExpand"
+    "snd"
+  apply default
+  apply (simp add: Aheap_subst  Aheap_cong[OF Aexp_subst_restr])[1]
+  apply (rule subst_Aeta_expand)  
+  sorry
+
+  abbreviation ccTransform where "ccTransform \<equiv> transform"
+
+  type_synonym tstate = "(AEnv \<times> (var \<Rightarrow> two) \<times> Arity)"
+
+  fixrec u_com :: "'a::cpo\<^sub>\<bottom> \<rightarrow> 'b::cpo\<^sub>\<bottom> \<rightarrow> ('a \<times> 'b)\<^sub>\<bottom>"
+    where "u_com\<cdot>(up\<cdot>x)\<cdot>(up\<cdot>y) = up\<cdot>(x, y)"
+  lemma u_com_strict[simp]: "u_com\<cdot>\<bottom>\<cdot>\<bottom> = \<bottom>" by fixrec_simp
+
+  definition env_u_com ::  "('c::type \<Rightarrow> 'a::cpo\<^sub>\<bottom>) \<Rightarrow> ('c \<Rightarrow> 'b::cpo\<^sub>\<bottom>) \<Rightarrow> ('c \<Rightarrow> ('a \<times> 'b)\<^sub>\<bottom>)"
+    where [simp]: "env_u_com e1 e2 x = u_com\<cdot>(e1 x)\<cdot>(e2 x)"
+  lemma env_u_com_delete: "env_u_com (env_delete x e1) (env_delete x e2) = env_delete x (env_u_com e1 e2)"
+    by (rule, case_tac "xa = x") auto
+  
+
+  fun conf_transform :: "tstate \<Rightarrow> conf \<Rightarrow> conf"
+  where "conf_transform (ae, ce,  a) (\<Gamma>, e, S) =
+    (map_transform rhsExpand (env_u_com ae ce) (map_transform ccTransform ae \<Gamma>), 
+     ccTransform a e,
+     restr_stack (edom ae) S)"
+
+  definition anal_env :: "(exp \<Rightarrow> 'a::cpo \<rightarrow> 'b::pcpo) \<Rightarrow> heap \<Rightarrow> (var \<Rightarrow> 'a\<^sub>\<bottom>) \<rightarrow> (var \<Rightarrow> 'b)"
+    where "anal_env f \<Gamma> = (\<Lambda> e. (\<lambda> x . fup\<cdot>(f (the (map_of \<Gamma> x)))\<cdot>(e x)))"
+
+  fun fstack :: "stack \<Rightarrow> future set \<rightarrow> future set"
+    where "fstack [] = (\<Lambda> f. f)"
+        | "fstack (Arg x # S) = (\<Lambda> f . fstack S \<cdot> (may_call x f))"
+        | "fstack (Upd x # S) = fstack S"
+        | "fstack (Dummy x # S) = fstack S"
+
+
+  definition const_on :: "('a \<Rightarrow> 'b) \<Rightarrow> 'a set \<Rightarrow> 'b \<Rightarrow> bool"
+    where "const_on f S x = (\<forall> y \<in> S . f y = x)"
+
+  lemma const_on_simp:
+   "const_on f S r \<Longrightarrow> x \<in> S \<Longrightarrow> f x = r"
+   by (simp add: const_on_def)
+
+  lemma const_onE[elim]: "const_on f S r ==> x : S ==> r = r' ==> f x = r'"     by (simp add: const_on_def)
+
+  lemma const_on_insert[simp]: "const_on f (insert x S) y \<longleftrightarrow> const_on f S y \<and> f x = y"
+    unfolding const_on_def by auto
+
+  lemma thunks_delete[simp]: "thunks (delete x \<Gamma>) = thunks \<Gamma> - {x}" sorry
+
+  fun prognosis :: "AEnv \<Rightarrow> Arity \<Rightarrow> conf \<Rightarrow> (var \<Rightarrow> two)"
+    where "prognosis ae a (\<Gamma>, e, S) = abstractPath (paths (anal_env fExp \<Gamma> \<cdot> ae) (fstack S \<cdot> (fExp e \<cdot> a)))"
+  lemmas prognosis.simps[simp del]
+
+  inductive consistent :: "tstate \<Rightarrow> conf \<Rightarrow> bool" where
+    consistentI[intro!]: 
+    "edom ae \<subseteq> domA \<Gamma> \<union> upds S
+    \<Longrightarrow> edom ce = edom ae
+    \<Longrightarrow> Astack (restr_stack (edom ae) S) \<sqsubseteq> a
+    \<Longrightarrow> aExp e \<cdot> a \<sqsubseteq> ae
+    \<Longrightarrow> prognosis ae a  (\<Gamma>, e, S) \<sqsubseteq> ce
+    \<Longrightarrow> (\<And> x. x \<in> thunks \<Gamma> \<Longrightarrow>  many \<sqsubseteq> ce x \<Longrightarrow> ae x = up\<cdot>0)
+    \<Longrightarrow> (\<And> x e'. map_of \<Gamma> x = Some e' \<Longrightarrow> x \<in> edom (prognosis ae a  (\<Gamma>, e, S)) \<Longrightarrow> fup\<cdot>(aExp e')\<cdot>(ae x) \<sqsubseteq> ae)
+    \<Longrightarrow> const_on ae (ap S) (up\<cdot>0)
+    \<Longrightarrow> consistent (ae, ce, a) (\<Gamma>, e, S)"  
+  inductive_cases consistentE[elim!]: "consistent (ae, ce, a) (\<Gamma>, e, S)"
+  
+  lemma foo:
+    fixes c c' R 
+    assumes "c \<Rightarrow>\<^sup>* c'" and "\<not> boring_step c'" and "consistent (ae,ce,a) c"
+    shows "\<exists>ae' ce' a'. consistent (ae',ce',a') c' \<and> conf_transform (ae,ce,a) c \<Rightarrow>\<^sub>G\<^sup>* conf_transform (ae',ce',a') c'"
+  using assms
+  proof(induction c c' arbitrary: ae ce a rule:step_induction)
+  case (app\<^sub>1 \<Gamma> e x S)
+    have " prognosis ae (inc\<cdot>a) (\<Gamma>, e, Arg x # S) = prognosis ae a (\<Gamma>, App e x, S)" sorry
+    with app\<^sub>1 have "consistent (ae, ce, inc\<cdot>a) (\<Gamma>, e, Arg x # S)"
+      by (auto simp add: join_below_iff fExp_App aExp_App)
+    moreover
+    have "conf_transform (ae, ce, a) (\<Gamma>, App e x, S) \<Rightarrow>\<^sub>G conf_transform (ae, ce, inc\<cdot>a) (\<Gamma>, e, Arg x # S)"
+      by simp rule
+    ultimately
+    show ?case by (blast del: consistentI consistentE)
+  next
+case (app\<^sub>2 \<Gamma> y e x S)
+  have "aExp (e[y ::= x])\<cdot>(pred\<cdot>a) \<sqsubseteq> ae" using app\<^sub>2
+    apply (auto simp add:  join_below_iff)
+    apply (rule below_trans[OF monofun_cfun_fun[OF aExp_subst_App_Lam]])
+    apply (auto simp add: aExp_App aExp_Lam join_below_iff)
+    done
+  moreover
+  have "fExp e[y::=x]\<cdot>(pred\<cdot>a) \<sqsubseteq> may_call x (fExp (Lam [y]. e)\<cdot>a)" sorry
+  hence "fstack S\<cdot>(fExp e[y::=x]\<cdot>(pred\<cdot>a)) \<sqsubseteq> fstack S\<cdot>(may_call x (fExp (Lam [y]. e)\<cdot>a))" by (rule monofun_cfun_arg)
+  hence "prognosis ae (pred\<cdot>a) (\<Gamma>, e[y::=x], S) \<sqsubseteq> prognosis ae a (\<Gamma>, (Lam [y]. e), Arg x # S)"
+    sorry
+  moreover
+  hence "edom (prognosis ae (pred\<cdot>a) (\<Gamma>, e[y::=x], S)) \<subseteq> edom (prognosis ae a (\<Gamma>, (Lam [y]. e), Arg x # S))" 
+    by (rule edom_mono)
+  ultimately
+  have "consistent (ae, ce, pred\<cdot>a) (\<Gamma>, e[y::=x], S)"  using app\<^sub>2
+    by (auto elim: below_trans)
+  moreover
+  have "conf_transform (ae, ce, a) (\<Gamma>, Lam [y]. e, Arg x # S) \<Rightarrow>\<^sub>G conf_transform (ae, ce, pred \<cdot> a) (\<Gamma>, e[y::=x], S)" by (simp add: subst_transform[symmetric]) rule
+  ultimately
+  show ?case by (blast  del: consistentI consistentE)
+next
+case (thunk \<Gamma> x e S)
+  hence "x \<in> thunks \<Gamma>" sorry
+
+  from thunk have "aExp (Var x)\<cdot>a \<sqsubseteq> ae" by auto
+  from below_trans[OF aExp_Var fun_belowD[OF this] ]
+  have "up\<cdot>a \<sqsubseteq> ae x".    
+  then obtain u where "ae x = up\<cdot>u" and "a \<sqsubseteq> u" by (cases "ae x") auto
+  hence [simp]: "x \<in> edom ae" by (simp add: edom_def)
+
+  have "Astack (restr_stack (edom ae) S) \<sqsubseteq> u" using thunk `a \<sqsubseteq> u` by (auto elim: below_trans)
+
+  have "x \<in> edom (prognosis ae a (\<Gamma>, Var x, S))" sorry
+  hence "fup\<cdot>(aExp e)\<cdot>(ae x) \<sqsubseteq> ae " using  thunk by blast
+  hence "aExp e\<cdot>u \<sqsubseteq> ae" using  `ae x = up\<cdot>u` by auto
+
+
+  show ?case
+  proof(cases "ce x" rule:two_cases)
+    case none
+    hence "ae x = \<bottom>"  using none thunk by (auto simp add: edom_def)
+    with `x \<in> edom ae` have False by (auto simp add: edom_def)
+    thus ?thesis..
+  next
+    case once
+
+    note `ae x = up\<cdot>u` `a \<sqsubseteq> u`
+    moreover
+
+    have "prognosis ae a (\<Gamma>, Var x, S) \<sqsubseteq> ce" using thunk by auto
+    hence "prognosis ae a (\<Gamma>, Var x, S) x \<sqsubseteq> once"
+      using once by (metis (mono_tags) fun_belowD)
+    hence "x \<notin> ap S" sorry
+    moreover
+
+    have *: "prognosis (env_delete x ae) u (delete x \<Gamma>, e, Upd x # S) \<sqsubseteq> prognosis ae a (\<Gamma>, Var x, S)"
+      sorry
+
+    from `prognosis ae a (\<Gamma>, Var x, S) x \<sqsubseteq> once`
+    have **:  "prognosis (env_delete x ae) u (delete x \<Gamma>, e, Upd x # S) x = \<bottom>" sorry
+  
+    have "prognosis (env_delete x ae) u (delete x \<Gamma>, e, Upd x # S) \<sqsubseteq> env_delete x ce"
+      using ** below_trans[OF * `prognosis ae a (\<Gamma>, Var x, S) \<sqsubseteq> ce`]
+      by (rule below_env_deleteI)
+    moreover
+
+    from **
+    have "(aExp e\<cdot>u) x = \<bottom>" sorry
+    hence "aExp e\<cdot>u \<sqsubseteq> env_delete x ae" using `aExp e\<cdot>u \<sqsubseteq> ae` by (metis below_env_deleteI)
+    moreover
+
+    {
+    fix x' e'
+    assume "map_of \<Gamma> x' = Some e'" and "x' \<noteq> x"
+    moreover
+    assume "x' \<in> edom (prognosis (env_delete x ae) u (delete x \<Gamma>, e, Upd x # S))"
+    hence "x' \<in> edom (prognosis ae a (\<Gamma>, Var x, S))" using edom_mono[OF *]..
+    ultimately
+    have "fup\<cdot>(aExp e')\<cdot>(ae x') \<sqsubseteq> ae" using thunk by auto
+    moreover
+    have "(fup\<cdot>(aExp e')\<cdot>(ae x')) x = \<bottom>" sorry
+    ultimately
+    have "fup\<cdot>(aExp e')\<cdot>(ae x') \<sqsubseteq> env_delete x ae" sorry
+    }
+    moreover
+
+    have "const_on ae (ap S) (up\<cdot>0)" using thunk by auto
+    hence "const_on (env_delete x ae) (ap S) (up\<cdot>0)" using `x \<notin>  ap S`
+      by (auto simp add: const_on_def env_delete_def)
+    ultimately
+
+    have "consistent (env_delete x ae, env_delete x ce, u) (delete x \<Gamma>, e, Upd x # S)" using thunk
+      by (auto simp add: join_below_iff insert_absorb elim:below_trans)
+     
+    moreover
+    
+    {
+    from  `map_of \<Gamma> x = Some e` `ae x = up\<cdot>u` once
+    have "map_of (map_transform rhsExpand (env_u_com ae ce) (map_transform ccTransform ae \<Gamma>)) x = Some (Aeta_expand u (transform u e))"
+      by (simp add: map_of_map_transform)
+    hence "(map_transform rhsExpand (env_u_com ae ce) (map_transform ccTransform ae \<Gamma>), Var x, restr_stack (edom ae) S) \<Rightarrow>\<^sub>G
+           (delete x (map_transform rhsExpand (env_u_com ae ce) (map_transform ccTransform ae \<Gamma>)), Aeta_expand u (ccTransform u e), Upd x # restr_stack (edom ae) S)"
+        by (auto simp add: env_u_com_delete  map_transform_delete delete_map_transform_env_delete insert_absorb)
+    also
+    have "\<dots> \<Rightarrow>\<^sub>G\<^sup>* (delete x (map_transform rhsExpand (env_u_com ae ce) (map_transform ccTransform ae \<Gamma>)), Aeta_expand u (ccTransform u e), restr_stack (edom ae) S)"
+      by (rule r_into_rtranclp, rule)
+    also
+    have "\<dots> \<Rightarrow>\<^sub>G\<^sup>* (delete x (map_transform rhsExpand (env_u_com ae ce) (map_transform ccTransform ae \<Gamma>)), ccTransform u e, restr_stack (edom ae) S)"
+      by (intro normal_trans Aeta_expand_correct `Astack (restr_stack (edom ae) S) \<sqsubseteq> u`)
+    finally(rtranclp_trans)
+    have "conf_transform (ae, ce, a) (\<Gamma>, Var x, S) \<Rightarrow>\<^sub>G\<^sup>* conf_transform (env_delete x ae, env_delete x ce, u) (delete x \<Gamma>, e, Upd x # S)"
+      by (auto simp add: env_u_com_delete  map_transform_delete delete_map_transform_env_delete insert_absorb)
+    }
+    ultimately
+    show ?thesis by (blast del: consistentI consistentE)
+
+
+  next
+    case many
+    have *: "prognosis ae 0 (delete x \<Gamma>, e, Upd x # S) \<sqsubseteq> prognosis ae a (\<Gamma>, Var x, S)" sorry
+
+    have "ae x = up\<cdot>0" using thunk many `x \<in> thunks \<Gamma>` by (auto)
+    hence "u = 0" using `ae x = up\<cdot>u` by simp
+    
+    have "prognosis ae 0 (delete x \<Gamma>, e, Upd x # S) \<sqsubseteq> ce" using * thunk by (auto elim: below_trans)
+    hence "consistent (ae, ce, 0) (delete x \<Gamma>, e, Upd x # S)" using thunk  `aExp e\<cdot>u \<sqsubseteq> ae` `u = 0` edom_mono[OF *]
+      by (auto simp add: join_below_iff)
+    moreover
+    from  `map_of \<Gamma> x = Some e` `ae x = up\<cdot>0` many
+    have "map_of (map_transform rhsExpand (env_u_com ae ce) (map_transform ccTransform ae \<Gamma>)) x = Some (transform 0 e)"
+      by (simp add: map_of_map_transform)
+    with `\<not> isLam e`
+    have "conf_transform (ae, ce, a) (\<Gamma>, Var x, S) \<Rightarrow>\<^sub>G conf_transform (ae, ce, 0) (delete x \<Gamma>, e, Upd x # S)"
+      by (auto simp add: map_transform_delete intro!: step.intros)
+    ultimately
+    show ?thesis by (blast del: consistentI consistentE)
+  next
+
+
+
+
+
+
+end
