Launchbury/SestoftGC.thy
@@ -1,0 +1,34 @@
+theory SestoftGC
+imports Sestoft 
+begin
+
+inductive gc_step :: "conf \<Rightarrow> conf \<Rightarrow> bool" (infix "\<Rightarrow>\<^sub>G" 50) where
+  normal:  "c \<Rightarrow> c' \<Longrightarrow> c \<Rightarrow>\<^sub>G c'"
+| drop:    "(\<Gamma>, e, S) \<Rightarrow>\<^sub>G (restrictA V \<Gamma>, e, S)"
+| dropUpd: "(\<Gamma>, e, Upd x # S) \<Rightarrow>\<^sub>G (\<Gamma>, e, S)"
+
+lemmas gc_step_intros[intro] =
+  normal[OF step.intros(1)] normal[OF step.intros(2)] normal[OF step.intros(3)]
+  normal[OF step.intros(4)] normal[OF step.intros(5)] drop dropUpd
+
+
+abbreviation gc_steps (infix "\<Rightarrow>\<^sub>G\<^sup>*" 50) where "gc_steps \<equiv> gc_step\<^sup>*\<^sup>*"
+
+lemma var_onceI:
+  assumes "map_of \<Gamma> x = Some e"
+  shows "(\<Gamma>, Var x, S) \<Rightarrow>\<^sub>G\<^sup>* (delete x \<Gamma>, e , S)"
+proof-
+  from assms 
+  have "(\<Gamma>, Var x, S) \<Rightarrow>\<^sub>G (delete x \<Gamma>, e , Upd x # S)"..
+  moreover
+  have "\<dots> \<Rightarrow>\<^sub>G  (delete x \<Gamma>, e , S)"..
+  ultimately
+  show ?thesis by (rule converse_rtranclp_into_rtranclp[OF _ r_into_rtranclp])
+qed
+
+lemma normal_trans:  "c \<Rightarrow>\<^sup>* c' \<Longrightarrow> c \<Rightarrow>\<^sub>G\<^sup>* c'"
+  by (induction rule:rtranclp_induct) (auto dest: normal)
+
+
+end
+
