Launchbury/Set_Cpo.thy
@@ -1,0 +1,38 @@
+theory Set_Cpo
+imports HOLCF
+begin
+
+instantiation set :: (type) below
+begin
+  definition below_set where "op \<sqsubseteq> = op \<subseteq>"
+instance..  
+end
+
+instance set :: (type) po
+  by default (auto simp add: below_set_def)
+
+lemma is_lub_fun:
+  "S <<| \<Union>S"
+  by(auto simp add: is_lub_def below_set_def is_ub_def)
+  
+instance set  :: (type) cpo
+  by default (rule exI, rule is_lub_fun)
+
+lemma minimal_set: "{} \<sqsubseteq> S"
+  unfolding below_set_def by simp
+
+instance set  :: (type) pcpo
+  by default (rule+, rule minimal_set)
+
+lemma set_contI:
+  assumes  "\<And> S. f (\<Union>S) = \<Union> (f ` S)"
+  shows "cont f"
+proof(rule contI)
+  case (goal1 Y)
+  have "f (\<Squnion> i. Y i) = \<Union> (range (\<lambda>i. f (Y i)))" 
+    using assms by (metis Set_Cpo.is_lub_fun image_image lub_eqI)
+  with is_lub_fun
+  show "range (\<lambda>i. f (Y i)) <<| f (\<Squnion> i. Y i)" by metis
+qed
+
+end
