Launchbury/Set_Cpo_Nominal.thy
@@ -1,0 +1,11 @@
+theory Set_Cpo_Nominal
+imports Set_Cpo "Nominal-HOLCF"
+begin
+
+instance set :: (pt) cont_pt
+  apply default
+  apply (rule set_contI)
+  apply perm_simp
+  apply (simp add : permute_set_eq_image)
+  done
+end
